Up to exp_match_ex1.

MQuinnIndProp.v
@@ -410,3 +410,71 @@ Proof. Abort.
    (list_head + 1), and since there is no rule allowing us to reduce n
    independently of modifying the list, R does not hold. *)
 
+Inductive reg_exp (T : Type) : Type :=
+  | EmptySet : reg_exp T
+  | EmptyStr : reg_exp T
+  | Char : T -> reg_exp T
+  | App : reg_exp T -> reg_exp T -> reg_exp T
+  | Union : reg_exp T -> reg_exp T -> reg_exp T
+  | Star : reg_exp T -> reg_exp T.
+
+Arguments EmptySet {T}.
+Arguments EmptyStr {T}.
+Arguments Char {T} _.
+Arguments App {T} _ _.
+Arguments Union {T} _ _.
+Arguments Star {T} _.
+
+Inductive exp_match {T} : list T -> reg_exp T -> Prop :=
+  | MEmpty : exp_match [] EmptyStr
+  | MChar : forall x, exp_match [x] (Char x)
+  | MApp : forall s1 re1 s2 re2,
+            exp_match s1 re1 ->
+            exp_match s2 re2 ->
+            exp_match (s1 ++ s2) (App re1 re2)
+  | MUnionL : forall s1 re1 re2,
+            exp_match s1 re1 ->
+            exp_match s1 (Union re1 re2)
+  | MUnionR : forall re1 s2 re2,
+            exp_match s2 re2 ->
+            exp_match s2 (Union re1 re2)
+  | MStar0 : forall re, exp_match [] (Star re)
+  | MStarApp : forall s1 s2 re,
+                  exp_match s1 re ->
+                  exp_match s2 (Star re) ->
+                  exp_match (s1 ++ s2) (Star re).
+
+Notation "s =~ re" := (exp_match s re) (at level 80).
+
+Example reg_exp_ex1 : [1] =~ Char 1.
+Proof. apply MChar. Qed.
+
+Example reg_exp_ex2 : [1; 2] =~ App (Char 1) (Char 2).
+Proof. apply (MApp [1] _ [2]). (* Notice how these align with
+                                  MApp forall s1 re1 s2 re2 above;
+                                  fourth wildcard underscore is implied. *)
+  - apply MChar.
+  - apply MChar.
+Qed.
+
+Example reg_exp_ex3 : ~ ([1;2] =~ Char 1).
+Proof. intros H. inversion H. Qed.
+
+Fixpoint reg_exp_of_list {T} (l : list T) :=
+  match l with
+  | [] => EmptyStr
+  | x :: l' => App (Char x) (reg_exp_of_list l')
+  end.
+
+Example reg_exp_ex4 : [1; 2; 3] =~ reg_exp_of_list [1; 2; 3].
+Proof. simpl. apply (MApp [1]). { apply MChar. } apply (MApp [2]).
+  { apply MChar. } apply (MApp[3]). { apply MChar. } apply MEmpty.
+Qed.
+
+Lemma MStar1 : forall T s (re : reg_exp T), s =~ re -> s =~ Star re.
+Proof.
+  intros T s re H. rewrite <- (app_nil_r _ s).
+  apply (MStarApp s [] re).
+  - apply H.
+  - apply MStar0.
+Qed.
